timing/i386Timing.v
@@ -6,17 +6,5 @@ Require Export NArith.
 Module i386Timing.
     Definition store := store.
     Definition stmt := stmt.
-
-    Definition time_of_stmt (s : option (N * stmt)) : nat :=
-        match s with None => 0 | Some (_, s') => match s' with
-        | Move _ _ => 2
-        | If _ _ _ => 6
-        | Jmp _ => 9
-        | _ => 0
-        end end.
-
     Definition empty_store : store := fun _ => VaN 0 32.
 End i386Timing.
-
-Module i386T := MakeTimingContents(i386Timing).
-Export i386T.
